changed nested loop2

BoogieLang/generated_example_proofs/nested_loop2_proofs/nested_loop2_proofs/nested_loop2_ast_cfg_proof.thy
@@ -16,8 +16,8 @@ abbreviation \<Lambda>1_local
   where
     "\<Lambda>1_local  \<equiv> ((append global_data.constants_vdecls global_data.globals_vdecls),(append nested_loop2_before_cfg_to_dag_prog.params_vdecls nested_loop2_before_cfg_to_dag_prog.locals_vdecls))"
 
-definition outer_body_bb1 
-  where "outer_body_bb1 \<equiv> 
+definition loop2_body_bb1 
+  where "loop2_body_bb1 \<equiv> 
                      (BigBlock None [] 
                      (Some (WhileWrapper 
                            (ParsedWhile (Some (BinOp (Var 1) Gt (Lit (LInt 0))))
@@ -25,22 +25,22 @@ definition outer_body_bb1
                             [BigBlock None [(Assign 1 (BinOp (Var 1) Sub (Lit (LInt 1))))] None None]))) 
                       None)"
 
-definition outer_body_bb2
-  where "outer_body_bb2 \<equiv> (BigBlock None [(Assign 0 (BinOp (Var 0) Sub (Lit (LInt 1))))] None None)"
+definition loop2_body_bb2
+  where "loop2_body_bb2 \<equiv> (BigBlock None [(Assign 0 (BinOp (Var 0) Sub (Lit (LInt 1))))] None None)"
 
-definition outer_body_bb1_unwrapped where
-  "outer_body_bb1_unwrapped \<equiv> 
+definition loop2_body_bb1_unwrapped where
+  "loop2_body_bb1_unwrapped \<equiv> 
                    (BigBlock None [] 
                    (Some (ParsedWhile (Some (BinOp (Var 1) Gt (Lit (LInt 0))))
                           [(BinOp (Var 1) Ge (Lit (LInt 0)))] 
                           [BigBlock None [(Assign 1 (BinOp (Var 1) Sub (Lit (LInt 1))))] None None])) 
                     None)"
 
-definition inner_body_bb1 
-  where "inner_body_bb1 \<equiv> (BigBlock None [(Assign 1 (BinOp (Var 1) Sub (Lit (LInt 1))))] None None)"
+definition loop3_body_bb1 
+  where "loop3_body_bb1 \<equiv> (BigBlock None [(Assign 1 (BinOp (Var 1) Sub (Lit (LInt 1))))] None None)"
 
-definition loop_only_bigblock0 where
-  "loop_only_bigblock0 \<equiv> 
+definition loop1_body_bb1 where
+  "loop1_body_bb1 \<equiv> 
                       (BigBlock None []
                       (Some (WhileWrapper 
                             (ParsedWhile (Some (BinOp (Var 0) Gt (Lit (LInt 0)))) 
@@ -54,8 +54,8 @@ definition loop_only_bigblock0 where
                              (BigBlock None [(Assign 0 (BinOp (Var 0) Sub (Lit (LInt 1))))] None None)]))) 
                        None)"
 
-definition bb0_unwrapped where
-  "bb0_unwrapped \<equiv> (BigBlock None []
+definition loop1_body_bb1_unwrapped where
+  "loop1_body_bb1_unwrapped \<equiv> (BigBlock None []
                     (Some (ParsedWhile (Some (BinOp (Var 0) Gt (Lit (LInt 0)))) 
                           [(BinOp (Var 0) Ge (Lit (LInt 0)))]
                           [(BigBlock None [] 
@@ -66,6 +66,45 @@ definition bb0_unwrapped where
                            None),
                            (BigBlock None [(Assign 0 (BinOp (Var 0) Sub (Lit (LInt 1))))] None None)])) 
                      None)"
+
+definition loop_only_bigblock0 where
+  "loop_only_bigblock0 \<equiv> 
+                      BigBlock None []
+                     (Some (WhileWrapper 
+                           (ParsedWhile (Some ((Lit (LBool True))))
+                            []
+                            [(BigBlock None []
+                             (Some (WhileWrapper 
+                                   (ParsedWhile (Some (BinOp (Var 0) Gt (Lit (LInt 0)))) 
+                                   [(BinOp (Var 0) Ge (Lit (LInt 0)))]
+                                   [(BigBlock None [] 
+                                    (Some (WhileWrapper 
+                                         (ParsedWhile (Some (BinOp (Var 1) Gt (Lit (LInt 0))))
+                                          [(BinOp (Var 1) Ge (Lit (LInt 0)))] 
+                                          [BigBlock None [(Assign 1 (BinOp (Var 1) Sub (Lit (LInt 1))))] None None]))) 
+                                     None),
+                                   (BigBlock None [(Assign 0 (BinOp (Var 0) Sub (Lit (LInt 1))))] None None)]))) 
+                              None)])))
+                       None"
+
+definition bb0_unwrapped where
+  "bb0_unwrapped \<equiv> BigBlock None []
+                     (Some 
+                           (ParsedWhile (Some ((Lit (LBool True))))
+                            []
+                            [(BigBlock None []
+                             (Some (WhileWrapper 
+                                   (ParsedWhile (Some (BinOp (Var 0) Gt (Lit (LInt 0)))) 
+                                   [(BinOp (Var 0) Ge (Lit (LInt 0)))]
+                                   [(BigBlock None [] 
+                                    (Some (WhileWrapper 
+                                         (ParsedWhile (Some (BinOp (Var 1) Gt (Lit (LInt 0))))
+                                          [(BinOp (Var 1) Ge (Lit (LInt 0)))] 
+                                          [BigBlock None [(Assign 1 (BinOp (Var 1) Sub (Lit (LInt 1))))] None None]))) 
+                                     None),
+                                   (BigBlock None [(Assign 0 (BinOp (Var 0) Sub (Lit (LInt 1))))] None None)]))) 
+                              None)]))
+                       None"
 
 definition empty_bb where
   "empty_bb \<equiv> (BigBlock None [] None None)"
@@ -89,8 +128,8 @@ proof -
     done
 qed
 
-lemma inner_body_bb1_local_rel:
-  assumes Red_bb: "red_bigblock A M \<Lambda>1_local \<Gamma> \<Omega> T (inner_body_bb1, cont0, (Normal ns1)) (reached_bb, reached_cont, reached_state)" 
+lemma loop3_body_bb1_local_rel:
+  assumes Red_bb: "red_bigblock A M \<Lambda>1_local \<Gamma> \<Omega> T (loop3_body_bb1, cont0, (Normal ns1)) (reached_bb, reached_cont, reached_state)" 
   and Red_impl: "(\<And> s2'.((red_cmd_list A M \<Lambda>1_local \<Gamma> \<Omega> nested_loop2_before_cfg_to_dag_prog.block_6 (Normal ns1) s2') \<Longrightarrow> (s2' \<noteq> Failure)))" 
   and trace_is_possible: "A,\<Lambda>1_local,\<Gamma>,\<Omega> \<turnstile> \<langle>(BinOp (Var 1) Gt (Lit (LInt 0))),ns1\<rangle> \<Down> BoolV True"
   shows "reached_state \<noteq> Failure  \<and>
@@ -100,19 +139,19 @@ proof -
     unfolding nested_loop2_before_cfg_to_dag_prog.block_6_def
     apply (rule guard_holds_push_through_assumption)
       apply (rule block_local_rel_generic)
-             apply (rule Rel_Main_test[of inner_body_bb1])
-             apply (simp add: inner_body_bb1_def)
+             apply (rule Rel_Main_test[of loop3_body_bb1])
+             apply (simp add: loop3_body_bb1_def)
             apply simp
            apply simp+
           apply (rule Red_bb)
          apply (rule push_through_assumption_test1, rule Red_impl)
             apply (simp add: nested_loop2_before_cfg_to_dag_prog.block_6_def)
-           apply (simp add: trace_is_possible inner_body_bb1_def)+
+           apply (simp add: trace_is_possible loop3_body_bb1_def)+
     done
 qed
 
-lemma outer_body_bb2_local_rel:
-  assumes Red_bb: "red_bigblock A M \<Lambda>1_local \<Gamma> \<Omega> T (outer_body_bb2 , KSeq bb0_unwrapped (KEndBlock KStop), (Normal ns1)) (reached_bb, reached_cont, reached_state)" 
+lemma loop2_body_bb2_local_rel:
+  assumes Red_bb: "red_bigblock A M \<Lambda>1_local \<Gamma> \<Omega> T (loop2_body_bb2 , cont0, (Normal ns1)) (reached_bb, reached_cont, reached_state)" 
   and Red_impl: "(\<And> s2'.((red_cmd_list A M \<Lambda>1_local \<Gamma> \<Omega> nested_loop2_before_cfg_to_dag_prog.block_7 (Normal ns1) s2') \<Longrightarrow> (s2' \<noteq> Failure)))" 
   and trace_is_possible: "A,\<Lambda>1_local,\<Gamma>,\<Omega> \<turnstile> \<langle>(BinOp (Var 1) Gt (Lit (LInt 0))), ns1\<rangle> \<Down> BoolV False"
   shows "reached_state \<noteq> Failure  \<and>
@@ -122,8 +161,8 @@ proof -
     unfolding nested_loop2_before_cfg_to_dag_prog.block_7_def 
     apply (rule guard_fails_push_through_assumption)
       apply (rule block_local_rel_generic)
-             apply (rule Rel_Main_test[of outer_body_bb2])
-             apply (simp add: outer_body_bb2_def)
+             apply (rule Rel_Main_test[of loop2_body_bb2])
+             apply (simp add: loop2_body_bb2_def)
             apply simp
            apply simp+
           apply (rule Red_bb)
@@ -134,7 +173,7 @@ proof -
             apply (rule neg_gt2)
           apply (rule trace_is_possible)
          apply simp
-        apply (simp add: outer_body_bb2_def)
+        apply (simp add: loop2_body_bb2_def)
         apply simp+
      apply (rule neg_gt2)
     apply (rule trace_is_possible)
@@ -145,8 +184,11 @@ qed
 lemma end_global_rel: 
   assumes Red_bb: "A,M,\<Lambda>1_local,\<Gamma>,\<Omega>,T \<turnstile> (empty_bb, KStop, (Normal ns1)) -n\<longrightarrow>^j (reached_bb, reached_cont, reached_state)"
   and cfg_is_correct: "\<And> m' s'. (red_cfg_multi A M \<Lambda>1_local \<Gamma> \<Omega> nested_loop2_before_cfg_to_dag_prog.proc_body ((Inl 9),(Normal ns1)) (m',s')) \<Longrightarrow> (s' \<noteq> Failure)"
+  and cfg_satisfies_post: "\<And>m' s'.
+                           (A,M,\<Lambda>1_local,\<Gamma>,\<Omega>,nested_loop2_before_cfg_to_dag_prog.proc_body \<turnstile>(Inl 9, Normal ns1) -n\<rightarrow>* (m', s')) \<Longrightarrow>
+                           is_final_config (m', s') \<Longrightarrow> (\<forall>ns_end. s' = Normal ns_end \<longrightarrow> list_all (expr_sat A \<Lambda>1_local \<Gamma> \<Omega> ns_end) nested_loop2_before_ast_cfg.post)"
   and trace_is_possible: "A,\<Lambda>1_local,\<Gamma>,\<Omega> \<turnstile> \<langle>(Lit (LBool True)), ns1\<rangle> \<Down> BoolV False"
-shows "(Ast.valid_configuration A \<Lambda>1_local \<Gamma> \<Omega> [] reached_bb reached_cont reached_state)"
+shows "(Ast.valid_configuration A \<Lambda>1_local \<Gamma> \<Omega> nested_loop2_before_ast_cfg.post reached_bb reached_cont reached_state)"
 proof -
   have node3_loc: "node_to_block nested_loop2_before_cfg_to_dag_prog.proc_body ! 9 = [(Assume (UnOp Not (Lit (LBool True))))]" 
     by (simp add: nested_loop2_before_cfg_to_dag_prog.block_9_def nested_loop2_before_cfg_to_dag_prog.node_9)
@@ -167,36 +209,43 @@ proof -
          defer
         apply (rule trace_is_possible)
        apply (rule nested_loop2_before_cfg_to_dag_prog.outEdges_9)
-      apply (rule cfg_is_correct, simp)
-     apply simp
-    apply (simp add: empty_bb_def)
+       apply (rule cfg_is_correct, simp)
+      apply (rule cfg_satisfies_post, blast)
+      apply simp
+     apply (simp add: empty_bb_def)
      apply (simp add: end_static)
     apply simp
     done
 qed
 
 
-lemma outer_body_bb2_global_rel:
-  assumes concrete_trace: "A,M,\<Lambda>1_local,\<Gamma>,\<Omega>,T \<turnstile> (outer_body_bb2, KSeq bb0_unwrapped (KEndBlock KStop), (Normal ns1)) -n\<longrightarrow>^j (reached_bb, reached_cont, reached_state)"
+lemma loop2_body_bb2_global_rel:
+  assumes concrete_trace: "A,M,\<Lambda>1_local,\<Gamma>,\<Omega>,T \<turnstile> (loop2_body_bb2, KSeq loop1_body_bb1_unwrapped (KEndBlock (KSeq bb0_unwrapped (KEndBlock KStop))), (Normal ns1)) -n\<longrightarrow>^j (reached_bb, reached_cont, reached_state)"
   and cfg_is_correct: "\<And> m' s'. (red_cfg_multi A M \<Lambda>1_local \<Gamma> \<Omega> nested_loop2_before_cfg_to_dag_prog.proc_body ((Inl 7),(Normal ns1)) (m',s')) \<Longrightarrow> (s' \<noteq> Failure)"
+  and cfg_satisfies_post: "\<And>m' s'.
+                           (A,M,\<Lambda>1_local,\<Gamma>,\<Omega>,nested_loop2_before_cfg_to_dag_prog.proc_body \<turnstile>(Inl 7, Normal ns1) -n\<rightarrow>* (m', s')) \<Longrightarrow>
+                           is_final_config (m', s') \<Longrightarrow> (\<forall>ns_end. s' = Normal ns_end \<longrightarrow> list_all (expr_sat A \<Lambda>1_local \<Gamma> \<Omega> ns_end) nested_loop2_before_ast_cfg.post)"
   and trace_is_possible: "A,\<Lambda>1_local,\<Gamma>,\<Omega> \<turnstile> \<langle>(BinOp (Var 1) Gt (Lit (LInt 0))), ns1\<rangle> \<Down> BoolV False"
   and loop_ih:
         "\<And>k ns1'. k < j \<Longrightarrow>
-        (A,M,\<Lambda>1_local,\<Gamma>,\<Omega>,T \<turnstile>(bb0_unwrapped, (KEndBlock KStop), Normal ns1') -n\<longrightarrow>^k (reached_bb, reached_cont, reached_state)) \<Longrightarrow>
+        (A,M,\<Lambda>1_local,\<Gamma>,\<Omega>,T \<turnstile>(loop1_body_bb1_unwrapped, (KEndBlock (KSeq bb0_unwrapped (KEndBlock KStop))), Normal ns1') -n\<longrightarrow>^k (reached_bb, reached_cont, reached_state)) \<Longrightarrow>
         (\<And> m' s'. (red_cfg_multi A M \<Lambda>1_local \<Gamma> \<Omega> nested_loop2_before_cfg_to_dag_prog.proc_body ((Inl 3),(Normal ns1')) (m',s')) \<Longrightarrow> (s' \<noteq> Failure)) \<Longrightarrow>
-        (Ast.valid_configuration A \<Lambda>1_local \<Gamma> \<Omega> [] reached_bb reached_cont reached_state)" 
-  shows "(Ast.valid_configuration A \<Lambda>1_local \<Gamma> \<Omega> [] reached_bb reached_cont reached_state)" 
+        (\<And>m' s'.
+                 (A,M,\<Lambda>1_local,\<Gamma>,\<Omega>,nested_loop2_before_cfg_to_dag_prog.proc_body \<turnstile>(Inl 3, Normal ns1') -n\<rightarrow>* (m', s')) \<Longrightarrow>
+                 is_final_config (m', s') \<Longrightarrow> (\<forall>ns_end. s' = Normal ns_end \<longrightarrow> list_all (expr_sat A \<Lambda>1_local \<Gamma> \<Omega> ns_end) nested_loop2_before_ast_cfg.post)) \<Longrightarrow>
+        (Ast.valid_configuration A \<Lambda>1_local \<Gamma> \<Omega> nested_loop2_before_ast_cfg.post reached_bb reached_cont reached_state)" 
+  shows "(Ast.valid_configuration A \<Lambda>1_local \<Gamma> \<Omega> nested_loop2_before_ast_cfg.post reached_bb reached_cont reached_state)" 
   using assms
 proof -
   have node5_loc: "node_to_block nested_loop2_before_cfg_to_dag_prog.proc_body ! 7 = [(Assume (BinOp (Lit (LInt 0)) Ge (Var 1))),(Assign 0 (BinOp (Var 0) Sub (Lit (LInt 1))))]" 
     by (simp add: nested_loop2_before_cfg_to_dag_prog.block_7_def nested_loop2_before_cfg_to_dag_prog.node_7)
   show ?thesis 
     apply (rule block_global_rel_generic)
-           apply (rule Rel_Main_test[of outer_body_bb2])
-             apply (simp add: outer_body_bb2_def)
+           apply (rule Rel_Main_test[of loop2_body_bb2])
+             apply (simp add: loop2_body_bb2_def)
             defer
           apply (rule assms(1))
-         apply (simp add: outer_body_bb2_def)
+         apply (simp add: loop2_body_bb2_def)
         apply (rule disjI2)
         apply (rule disjI2)
         apply (rule conjI)
@@ -207,44 +256,53 @@ proof -
          apply (rule neg_gt2)
         apply (rule trace_is_possible)
        apply (rule assms(2))
-       apply simp+
+         apply simp+
+        apply (rule cfg_satisfies_post, blast)
+        apply simp+
      apply (simp add: nested_loop2_before_cfg_to_dag_prog.node_7)
-     apply (rule outer_body_bb2_local_rel)
+     apply (rule loop2_body_bb2_local_rel)
        apply assumption
       apply simp
      apply (rule trace_is_possible)
-    apply (erule allE[where x=3])
+    apply (erule allE[where x=3])+
     apply (simp add: nested_loop2_before_cfg_to_dag_prog.outEdges_7)
     apply (simp add: member_rec(1))
     apply (rule loop_ih)
-      apply simp+
+        apply simp+
+     apply blast+
     done
 qed
 
 
-lemma inner_loop_body_global_rel:
+lemma loop3_body_bb1_global_rel:
   assumes j_step_ast_trace: 
-          "A,M,\<Lambda>1_local,\<Gamma>,\<Omega>,T \<turnstile> (inner_body_bb1, (KSeq outer_body_bb1_unwrapped (KEndBlock (KSeq outer_body_bb2 (KSeq bb0_unwrapped (KEndBlock KStop))))), Normal ns1) -n\<longrightarrow>^j 
+          "A,M,\<Lambda>1_local,\<Gamma>,\<Omega>,T \<turnstile> (loop3_body_bb1, (KSeq loop2_body_bb1_unwrapped (KEndBlock (KSeq loop2_body_bb2 (KSeq loop1_body_bb1_unwrapped (KEndBlock (KSeq bb0_unwrapped (KEndBlock KStop))))))), Normal ns1) -n\<longrightarrow>^j 
                                  (reached_bb, reached_cont, reached_state)"
   and cfg_is_correct: "\<And> m' s'. (red_cfg_multi A M \<Lambda>1_local \<Gamma> \<Omega> nested_loop2_before_cfg_to_dag_prog.proc_body ((Inl 6),(Normal ns1)) (m',s')) \<Longrightarrow> (s' \<noteq> Failure)"
+  and cfg_satisfies_post: "\<And>m' s'.
+                           (A,M,\<Lambda>1_local,\<Gamma>,\<Omega>,nested_loop2_before_cfg_to_dag_prog.proc_body \<turnstile>(Inl 6, Normal ns1) -n\<rightarrow>* (m', s')) \<Longrightarrow>
+                           is_final_config (m', s') \<Longrightarrow> (\<forall>ns_end. s' = Normal ns_end \<longrightarrow> list_all (expr_sat A \<Lambda>1_local \<Gamma> \<Omega> ns_end) nested_loop2_before_ast_cfg.post)"
   and trace_is_possible: "A,\<Lambda>1_local,\<Gamma>,\<Omega> \<turnstile> \<langle>(BinOp (Var 1) Gt (Lit (LInt 0))),ns1\<rangle> \<Down> BoolV True"
   and loop_ih:
         "\<And>k ns1''. k < j \<Longrightarrow>
-        (A,M,\<Lambda>1_local,\<Gamma>,\<Omega>,T \<turnstile>(outer_body_bb1_unwrapped, (KEndBlock (KSeq outer_body_bb2 (KSeq bb0_unwrapped (KEndBlock KStop)))), Normal ns1'') -n\<longrightarrow>^k (reached_bb, reached_cont, reached_state)) \<Longrightarrow>
+        (A,M,\<Lambda>1_local,\<Gamma>,\<Omega>,T \<turnstile>(loop2_body_bb1_unwrapped, (KEndBlock (KSeq loop2_body_bb2 (KSeq loop1_body_bb1_unwrapped (KEndBlock (KSeq bb0_unwrapped (KEndBlock KStop)))))), Normal ns1'') -n\<longrightarrow>^k (reached_bb, reached_cont, reached_state)) \<Longrightarrow>
         (\<And> m' s'. (red_cfg_multi A M \<Lambda>1_local \<Gamma> \<Omega> nested_loop2_before_cfg_to_dag_prog.proc_body ((Inl 5),(Normal ns1'')) (m',s')) \<Longrightarrow> (s' \<noteq> Failure)) \<Longrightarrow>
-        (Ast.valid_configuration A \<Lambda>1_local \<Gamma> \<Omega> [] reached_bb reached_cont reached_state)" 
-  shows "(Ast.valid_configuration A \<Lambda>1_local \<Gamma> \<Omega> [] reached_bb reached_cont reached_state)"
+        (\<And>m' s'.
+                   (A,M,\<Lambda>1_local,\<Gamma>,\<Omega>,nested_loop2_before_cfg_to_dag_prog.proc_body \<turnstile>(Inl 5, Normal ns1'') -n\<rightarrow>* (m', s')) \<Longrightarrow>
+                   is_final_config (m', s') \<Longrightarrow> (\<forall>ns_end. s' = Normal ns_end \<longrightarrow> list_all (expr_sat A \<Lambda>1_local \<Gamma> \<Omega> ns_end) nested_loop2_before_ast_cfg.post)) \<Longrightarrow>
+        (Ast.valid_configuration A \<Lambda>1_local \<Gamma> \<Omega> nested_loop2_before_ast_cfg.post reached_bb reached_cont reached_state)" 
+  shows "(Ast.valid_configuration A \<Lambda>1_local \<Gamma> \<Omega> nested_loop2_before_ast_cfg.post reached_bb reached_cont reached_state)"
 proof -
   have node5_loc: "node_to_block nested_loop2_before_cfg_to_dag_prog.proc_body ! 6 = 
                    [(Assume (BinOp (Var 1) Gt (Lit (LInt 0)))),(Assign 1 (BinOp (Var 1) Sub (Lit (LInt 1))))]" 
     by (simp add: nested_loop2_before_cfg_to_dag_prog.block_6_def nested_loop2_before_cfg_to_dag_prog.node_6)
   show ?thesis 
     apply (rule block_global_rel_generic)
-           apply (rule Rel_Main_test[of inner_body_bb1])
-             apply (simp add: inner_body_bb1_def)
+           apply (rule Rel_Main_test[of loop3_body_bb1])
+             apply (simp add: loop3_body_bb1_def)
             defer
           apply (rule assms(1))
-         apply (simp add: inner_body_bb1_def)
+         apply (simp add: loop3_body_bb1_def)
         apply (rule disjI2)
         apply (rule disjI1)
         apply (rule conjI)
@@ -253,31 +311,40 @@ proof -
          apply simp
         apply (rule trace_is_possible)
        apply (rule assms(2))
-       apply simp+
+         apply simp+
+        apply (rule cfg_satisfies_post, blast)
+        apply simp+
      apply (simp add: nested_loop2_before_cfg_to_dag_prog.node_6)
-     apply (rule inner_body_bb1_local_rel)
+     apply (rule loop3_body_bb1_local_rel)
        apply assumption
       apply simp
      apply (rule trace_is_possible)
 
-    apply (erule allE[where x=5])
+    apply (erule allE[where x=5])+
     apply (simp add: nested_loop2_before_cfg_to_dag_prog.outEdges_6)
     apply (simp add: member_rec(1))
     apply (rule loop_ih)
-      apply simp+
+        apply simp+
+     apply blast+
     done
 qed
 
 
-lemma inner_loop_head_global_rel:
-  assumes j_step_ast_trace: "A,M,\<Lambda>1_local,\<Gamma>,\<Omega>,T \<turnstile> (outer_body_bb1_unwrapped, (KEndBlock (KSeq outer_body_bb2 (KSeq bb0_unwrapped (KEndBlock KStop)))), Normal ns1) -n\<longrightarrow>^j (reached_bb, reached_cont, reached_state)"
+lemma loop2_body_bb1_unwrapped_global_rel:
+  assumes j_step_ast_trace: "A,M,\<Lambda>1_local,\<Gamma>,\<Omega>,T \<turnstile> (loop2_body_bb1_unwrapped, (KEndBlock (KSeq loop2_body_bb2 (KSeq loop1_body_bb1_unwrapped (KEndBlock (KSeq bb0_unwrapped (KEndBlock KStop)))))), Normal ns1) -n\<longrightarrow>^j (reached_bb, reached_cont, reached_state)"
   and cfg_is_correct: "\<And> m' s'. (red_cfg_multi A M \<Lambda>1_local \<Gamma> \<Omega> nested_loop2_before_cfg_to_dag_prog.proc_body ((Inl 5),(Normal ns1)) (m',s')) \<Longrightarrow> (s' \<noteq> Failure)"
+  and cfg_satisfies_post: "\<And>m' s'.
+                           (A,M,\<Lambda>1_local,\<Gamma>,\<Omega>,nested_loop2_before_cfg_to_dag_prog.proc_body \<turnstile>(Inl 5, Normal ns1) -n\<rightarrow>* (m', s')) \<Longrightarrow>
+                           is_final_config (m', s') \<Longrightarrow> (\<forall>ns_end. s' = Normal ns_end \<longrightarrow> list_all (expr_sat A \<Lambda>1_local \<Gamma> \<Omega> ns_end) nested_loop2_before_ast_cfg.post)"
   and loop_ih:
         "\<And>k ns1'. k < j \<Longrightarrow>
-        (A,M,\<Lambda>1_local,\<Gamma>,\<Omega>,T \<turnstile>(bb0_unwrapped, KEndBlock KStop, Normal ns1') -n\<longrightarrow>^k (reached_bb, reached_cont, reached_state)) \<Longrightarrow>
+        (A,M,\<Lambda>1_local,\<Gamma>,\<Omega>,T \<turnstile>(loop1_body_bb1_unwrapped, (KEndBlock (KSeq bb0_unwrapped (KEndBlock KStop))), Normal ns1') -n\<longrightarrow>^k (reached_bb, reached_cont, reached_state)) \<Longrightarrow>
         (\<And> m' s'. (red_cfg_multi A M \<Lambda>1_local \<Gamma> \<Omega> nested_loop2_before_cfg_to_dag_prog.proc_body ((Inl 3),(Normal ns1')) (m',s')) \<Longrightarrow> (s' \<noteq> Failure)) \<Longrightarrow>
-        (Ast.valid_configuration A \<Lambda>1_local \<Gamma> \<Omega> [] reached_bb reached_cont reached_state)" 
-  shows "(Ast.valid_configuration A \<Lambda>1_local \<Gamma> \<Omega> [] reached_bb reached_cont reached_state)"
+        (\<And>m' s'.
+                   (A,M,\<Lambda>1_local,\<Gamma>,\<Omega>,nested_loop2_before_cfg_to_dag_prog.proc_body \<turnstile>(Inl 3, Normal ns1') -n\<rightarrow>* (m', s')) \<Longrightarrow>
+                   is_final_config (m', s') \<Longrightarrow> (\<forall>ns_end. s' = Normal ns_end \<longrightarrow> list_all (expr_sat A \<Lambda>1_local \<Gamma> \<Omega> ns_end) nested_loop2_before_ast_cfg.post)) \<Longrightarrow>
+        (Ast.valid_configuration A \<Lambda>1_local \<Gamma> \<Omega> nested_loop2_before_ast_cfg.post reached_bb reached_cont reached_state)" 
+  shows "(Ast.valid_configuration A \<Lambda>1_local \<Gamma> \<Omega> nested_loop2_before_ast_cfg.post reached_bb reached_cont reached_state)"
   using assms
 proof (induction j arbitrary: ns1 rule: less_induct)
   case (less j)
@@ -290,17 +357,18 @@ proof (induction j arbitrary: ns1 rule: less_induct)
     case (Suc j')
     show ?thesis
       apply (rule block_global_rel_loop_head)
-              apply (rule Rel_Invs[of outer_body_bb1_unwrapped _ _ _ nested_loop2_before_cfg_to_dag_prog.block_5])
-              apply (simp add: outer_body_bb1_unwrapped_def nested_loop2_before_cfg_to_dag_prog.block_5_def)
+              apply (rule Rel_Invs[of loop2_body_bb1_unwrapped _ _ _ nested_loop2_before_cfg_to_dag_prog.block_5])
+              apply (simp add: loop2_body_bb1_unwrapped_def nested_loop2_before_cfg_to_dag_prog.block_5_def)
              apply (rule less(2))
             apply (rule less(3), simp)
+           apply (rule less(4), blast)
            apply simp
-           apply (simp add: outer_body_bb1_unwrapped_def)
+           apply (simp add: loop2_body_bb1_unwrapped_def)
           apply simp
          apply (rule block_local_rel_loop_head)
-             apply (rule Rel_Invs[of outer_body_bb1_unwrapped])
-             apply (simp add: outer_body_bb1_unwrapped_def)
-            apply (simp add: outer_body_bb1_unwrapped_def)
+             apply (rule Rel_Invs[of loop2_body_bb1_unwrapped])
+             apply (simp add: loop2_body_bb1_unwrapped_def)
+            apply (simp add: loop2_body_bb1_unwrapped_def)
            apply (simp)
           apply (rule nested_loop2_before_cfg_to_dag_prog.block_5_def)
          apply (simp, simp)
@@ -308,27 +376,29 @@ proof (induction j arbitrary: ns1 rule: less_induct)
       apply(rule disjE)
         apply assumption
 
-       apply (erule allE[where x = 6])
+       apply (erule allE[where x = 6])+
        apply (simp add:nested_loop2_before_cfg_to_dag_prog.outEdges_5)
        apply (simp add:member_rec(1))
        apply (rule conjE)
         apply assumption
        apply simp
-       apply (rule inner_loop_body_global_rel) 
-          apply (simp add: inner_body_bb1_def)
-         apply simp
+       apply (rule loop3_body_bb1_global_rel) 
+          apply (simp add: loop3_body_bb1_def)
+          apply simp
+         apply blast
         apply assumption
        apply (rule less.IH)
          apply (rule strictly_smaller_helper2)
            apply assumption
           apply assumption
          apply assumption
-        apply assumption
-       apply (rule less.prems(3))
+         apply assumption
+        apply blast
+       apply (rule less.prems(4))
          apply (rule strictly_smaller_helper3)
            apply assumption+
 
-      apply (erule allE[where x = 7])
+      apply (erule allE[where x = 7])+
       apply (simp add:nested_loop2_before_cfg_to_dag_prog.outEdges_5)
       apply (simp add:member_rec(1))
       apply (rule conjE)
@@ -339,44 +409,207 @@ proof (induction j arbitrary: ns1 rule: less_induct)
           apply assumption
          apply simp
          apply blast
+        apply blast
         apply simp
-       apply assumption
-      apply (rule outer_body_bb2_global_rel)
+      apply (rule loop2_body_bb2_global_rel)
          apply assumption+
-      apply (rule less.prems(3))
+      apply (rule less.prems(4))
         apply (rule strictly_smaller_helper4)
           apply assumption+
       done
   qed
 qed
 
-lemma inner_loop_head_global_rel_wrapped:
-  assumes j_step_ast_trace: "A,M,\<Lambda>1_local,\<Gamma>,\<Omega>,T \<turnstile> (outer_body_bb1, (KSeq outer_body_bb2 (KSeq bb0_unwrapped (KEndBlock KStop))), Normal ns1) -n\<longrightarrow>^j (reached_bb, reached_cont, reached_state)"
+lemma loop2_body_bb1_wrapped_global_rel:
+  assumes j_step_ast_trace: "A,M,\<Lambda>1_local,\<Gamma>,\<Omega>,T \<turnstile> (loop2_body_bb1, (KSeq loop2_body_bb2 (KSeq loop1_body_bb1_unwrapped (KEndBlock (KSeq bb0_unwrapped (KEndBlock KStop))))), Normal ns1) -n\<longrightarrow>^j (reached_bb, reached_cont, reached_state)"
   and cfg_is_correct: "\<And> m' s'. (red_cfg_multi A M \<Lambda>1_local \<Gamma> \<Omega> nested_loop2_before_cfg_to_dag_prog.proc_body ((Inl 5),(Normal ns1)) (m',s')) \<Longrightarrow> (s' \<noteq> Failure)"
+  and cfg_satisfies_post: "\<And>m' s'.
+                           (A,M,\<Lambda>1_local,\<Gamma>,\<Omega>,nested_loop2_before_cfg_to_dag_prog.proc_body \<turnstile>(Inl 5, Normal ns1) -n\<rightarrow>* (m', s')) \<Longrightarrow>
+                           is_final_config (m', s') \<Longrightarrow> (\<forall>ns_end. s' = Normal ns_end \<longrightarrow> list_all (expr_sat A \<Lambda>1_local \<Gamma> \<Omega> ns_end) nested_loop2_before_ast_cfg.post)"
   and loop_ih:
         "\<And>k ns1'. k < j \<Longrightarrow>
-        (A,M,\<Lambda>1_local,\<Gamma>,\<Omega>,T \<turnstile>(bb0_unwrapped, KEndBlock KStop, Normal ns1') -n\<longrightarrow>^k (reached_bb, reached_cont, reached_state)) \<Longrightarrow>
+        (A,M,\<Lambda>1_local,\<Gamma>,\<Omega>,T \<turnstile>(loop1_body_bb1_unwrapped, (KEndBlock (KSeq bb0_unwrapped (KEndBlock KStop))), Normal ns1') -n\<longrightarrow>^k (reached_bb, reached_cont, reached_state)) \<Longrightarrow>
         (\<And> m' s'. (red_cfg_multi A M \<Lambda>1_local \<Gamma> \<Omega> nested_loop2_before_cfg_to_dag_prog.proc_body ((Inl 3),(Normal ns1')) (m',s')) \<Longrightarrow> (s' \<noteq> Failure)) \<Longrightarrow>
-        (Ast.valid_configuration A \<Lambda>1_local \<Gamma> \<Omega> [] reached_bb reached_cont reached_state)" 
-  shows "(Ast.valid_configuration A \<Lambda>1_local \<Gamma> \<Omega> [] reached_bb reached_cont reached_state)"
-  apply (rule ending3)
+        (\<And>m' s'.
+                   (A,M,\<Lambda>1_local,\<Gamma>,\<Omega>,nested_loop2_before_cfg_to_dag_prog.proc_body \<turnstile>(Inl 3, Normal ns1') -n\<rightarrow>* (m', s')) \<Longrightarrow>
+                   is_final_config (m', s') \<Longrightarrow> (\<forall>ns_end. s' = Normal ns_end \<longrightarrow> list_all (expr_sat A \<Lambda>1_local \<Gamma> \<Omega> ns_end) nested_loop2_before_ast_cfg.post)) \<Longrightarrow>
+        (Ast.valid_configuration A \<Lambda>1_local \<Gamma> \<Omega> nested_loop2_before_ast_cfg.post reached_bb reached_cont reached_state)" 
+  shows "(Ast.valid_configuration A \<Lambda>1_local \<Gamma> \<Omega> nested_loop2_before_ast_cfg.post reached_bb reached_cont reached_state)"
+  apply (rule ending_after_unwrapping)
      apply (rule j_step_ast_trace)
-    apply (simp add: outer_body_bb1_def)
+    apply (simp add: loop2_body_bb1_def)
     apply (rule cfg_is_correct, simp)
+   apply (rule cfg_satisfies_post, blast)
    apply simp
-  apply (rule inner_loop_head_global_rel)
-    apply (simp add: outer_body_bb1_unwrapped_def)
-   apply assumption
+  apply (rule loop2_body_bb1_unwrapped_global_rel)
+    apply (simp add: loop2_body_bb1_unwrapped_def)
+    apply assumption
+   apply blast
   apply (rule loop_ih)
     apply (rule strictly_smaller_helper2)
      apply assumption+
   done
 
-lemma outer_loop_head_global_rel:
+lemma loop1_body_bb1_unwrapped_global_rel:
+  assumes j_step_ast_trace: 
+    "A,M,\<Lambda>1_local,\<Gamma>,\<Omega>,T \<turnstile> (loop1_body_bb1_unwrapped, (KEndBlock (KSeq bb0_unwrapped (KEndBlock KStop))), Normal ns1) -n\<longrightarrow>^j (reached_bb, reached_cont, reached_state)"
+  and cfg_is_correct: "\<And> m' s'. (red_cfg_multi A M \<Lambda>1_local \<Gamma> \<Omega> nested_loop2_before_cfg_to_dag_prog.proc_body ((Inl 3),(Normal ns1)) (m',s')) \<Longrightarrow> (s' \<noteq> Failure)"
+  and cfg_satisfies_post: "\<And>m' s'.
+                           (A,M,\<Lambda>1_local,\<Gamma>,\<Omega>,nested_loop2_before_cfg_to_dag_prog.proc_body \<turnstile>(Inl 3, Normal ns1) -n\<rightarrow>* (m', s')) \<Longrightarrow>
+                           is_final_config (m', s') \<Longrightarrow> (\<forall>ns_end. s' = Normal ns_end \<longrightarrow> list_all (expr_sat A \<Lambda>1_local \<Gamma> \<Omega> ns_end) nested_loop2_before_ast_cfg.post)"
+  and loop_ih:
+        "\<And>k ns1'. k < j \<Longrightarrow>
+        (A,M,\<Lambda>1_local,\<Gamma>,\<Omega>,T \<turnstile>(bb0_unwrapped, KEndBlock KStop, Normal ns1') -n\<longrightarrow>^k (reached_bb, reached_cont, reached_state)) \<Longrightarrow>
+        (\<And> m' s'. (red_cfg_multi A M \<Lambda>1_local \<Gamma> \<Omega> nested_loop2_before_cfg_to_dag_prog.proc_body ((Inl 1),(Normal ns1')) (m',s')) \<Longrightarrow> (s' \<noteq> Failure)) \<Longrightarrow>
+        (\<And>m' s'.
+                   (A,M,\<Lambda>1_local,\<Gamma>,\<Omega>,nested_loop2_before_cfg_to_dag_prog.proc_body \<turnstile>(Inl 1, Normal ns1') -n\<rightarrow>* (m', s')) \<Longrightarrow>
+                   is_final_config (m', s') \<Longrightarrow> (\<forall>ns_end. s' = Normal ns_end \<longrightarrow> list_all (expr_sat A \<Lambda>1_local \<Gamma> \<Omega> ns_end) nested_loop2_before_ast_cfg.post)) \<Longrightarrow>
+        (Ast.valid_configuration A \<Lambda>1_local \<Gamma> \<Omega> nested_loop2_before_ast_cfg.post reached_bb reached_cont reached_state)" 
+  shows "(Ast.valid_configuration A \<Lambda>1_local \<Gamma> \<Omega> nested_loop2_before_ast_cfg.post reached_bb reached_cont reached_state)"
+  using assms 
+proof (induction j arbitrary: ns1 rule: less_induct)
+  case (less j)
+  then show ?case 
+  proof (cases j)
+    case 0
+    then show ?thesis
+      using valid_configuration_def less.prems(1) by fastforce
+  next
+    case (Suc j')
+    show ?thesis
+      apply (rule block_global_rel_loop_head) 
+              apply (rule Rel_Invs[of loop1_body_bb1_unwrapped])
+              apply (simp add: loop1_body_bb1_unwrapped_def)
+             apply (rule less(2))
+            apply (rule less(3), simp)
+           apply (rule less(4), blast)
+           apply simp
+           apply (simp add: loop1_body_bb1_unwrapped_def)
+          apply simp
+         apply (rule block_local_rel_loop_head)
+              apply (rule Rel_Invs[of loop1_body_bb1_unwrapped])
+              apply (simp add: loop1_body_bb1_unwrapped_def)
+            apply (simp add: loop1_body_bb1_unwrapped_def)
+           apply (simp, simp, simp)
+       apply (simp add: nested_loop2_before_cfg_to_dag_prog.node_3)
+       apply (simp add: nested_loop2_before_cfg_to_dag_prog.block_3_def)
+      apply(rule disjE)
+        apply assumption
+    
+       apply (erule allE[where x = 4])+
+       apply (simp add: nested_loop2_before_cfg_to_dag_prog.outEdges_3)
+       apply (simp add:member_rec(1))
+       apply (rule conjE)
+        apply assumption
+       apply simp
+       apply (rule loop2_body_bb1_wrapped_global_rel)
+         apply (simp add: loop2_body_bb1_def loop2_body_bb2_def)
+        apply (rule correctness_propagates_through_assumption2)
+            apply assumption
+           apply (simp add: nested_loop2_before_cfg_to_dag_prog.node_4)
+           apply (simp add: nested_loop2_before_cfg_to_dag_prog.block_4_def)
+          apply assumption
+         apply (simp add: nested_loop2_before_cfg_to_dag_prog.outEdges_4)
+         apply (simp add: member_rec)
+         apply assumption
+        apply (rule correctness_propagates_through_assumption4)
+             apply blast
+            apply (simp add: nested_loop2_before_cfg_to_dag_prog.node_4)
+            apply (simp add: nested_loop2_before_cfg_to_dag_prog.block_4_def)
+           apply simp
+          apply (simp add: nested_loop2_before_cfg_to_dag_prog.outEdges_4)
+          apply (simp add: member_rec)
+         apply simp+
+       apply (rule less.IH)
+         apply (rule strictly_smaller_helper2)
+           apply assumption
+          apply assumption
+         apply assumption
+         apply assumption
+        apply blast
+       apply (rule less.prems(4))
+         apply (rule strictly_smaller_helper3)
+           apply assumption+
+
+      apply (erule allE[where x = 8])+
+      apply (simp add:nested_loop2_before_cfg_to_dag_prog.outEdges_3)
+      apply (simp add:member_rec(1))
+      apply (rule conjE)
+       apply assumption
+      apply simp
+      apply (rule ending_after_skipping_endblock2)
+           apply assumption
+          apply assumption
+         apply simp
+         apply blast
+        apply blast
+        apply simp
+      apply (rule less(5))
+        apply (rule smaller_helper5)
+         apply assumption
+        apply assumption
+       apply assumption
+      apply (rule correctness_propagates_through_assumption)
+           apply assumption
+          apply (simp add: nested_loop2_before_cfg_to_dag_prog.node_8)
+          apply (simp add: nested_loop2_before_cfg_to_dag_prog.block_8_def)
+         apply (rule neg_gt2)
+        apply assumption  
+       apply (simp add: nested_loop2_before_cfg_to_dag_prog.outEdges_8)
+       apply (simp add: member_rec)
+       apply simp
+      apply (rule correctness_propagates_through_assumption3)
+            apply blast
+           apply (simp add: nested_loop2_before_cfg_to_dag_prog.node_8)
+           apply (simp add: nested_loop2_before_cfg_to_dag_prog.block_8_def)
+          apply (rule neg_gt2)
+         apply simp
+        apply (simp add: nested_loop2_before_cfg_to_dag_prog.outEdges_8)
+        apply (simp add: member_rec)
+       apply simp+
+      done
+  qed
+qed
+
+lemma loop1_body_bb1_wrapped_global_rel:
+  assumes j_step_ast_trace: 
+    "A,M,\<Lambda>1_local,\<Gamma>,\<Omega>,T \<turnstile> (loop1_body_bb1, (KSeq bb0_unwrapped (KEndBlock KStop)), Normal ns1) -n\<longrightarrow>^j (reached_bb, reached_cont, reached_state)"
+  and cfg_is_correct: "\<And> m' s'. (red_cfg_multi A M \<Lambda>1_local \<Gamma> \<Omega> nested_loop2_before_cfg_to_dag_prog.proc_body ((Inl 3),(Normal ns1)) (m',s')) \<Longrightarrow> (s' \<noteq> Failure)"
+  and cfg_satisfies_post: "\<And>m' s'.
+                           (A,M,\<Lambda>1_local,\<Gamma>,\<Omega>,nested_loop2_before_cfg_to_dag_prog.proc_body \<turnstile>(Inl 3, Normal ns1) -n\<rightarrow>* (m', s')) \<Longrightarrow>
+                           is_final_config (m', s') \<Longrightarrow> (\<forall>ns_end. s' = Normal ns_end \<longrightarrow> list_all (expr_sat A \<Lambda>1_local \<Gamma> \<Omega> ns_end) nested_loop2_before_ast_cfg.post)"
+  and loop_ih:
+        "\<And>k ns1'. k < j \<Longrightarrow>
+        (A,M,\<Lambda>1_local,\<Gamma>,\<Omega>,T \<turnstile>(bb0_unwrapped, KEndBlock KStop, Normal ns1') -n\<longrightarrow>^k (reached_bb, reached_cont, reached_state)) \<Longrightarrow>
+        (\<And> m' s'. (red_cfg_multi A M \<Lambda>1_local \<Gamma> \<Omega> nested_loop2_before_cfg_to_dag_prog.proc_body ((Inl 1),(Normal ns1')) (m',s')) \<Longrightarrow> (s' \<noteq> Failure)) \<Longrightarrow>
+        (\<And>m' s'.
+                   (A,M,\<Lambda>1_local,\<Gamma>,\<Omega>,nested_loop2_before_cfg_to_dag_prog.proc_body \<turnstile>(Inl 1, Normal ns1') -n\<rightarrow>* (m', s')) \<Longrightarrow>
+                   is_final_config (m', s') \<Longrightarrow> (\<forall>ns_end. s' = Normal ns_end \<longrightarrow> list_all (expr_sat A \<Lambda>1_local \<Gamma> \<Omega> ns_end) nested_loop2_before_ast_cfg.post)) \<Longrightarrow>
+        (Ast.valid_configuration A \<Lambda>1_local \<Gamma> \<Omega> nested_loop2_before_ast_cfg.post reached_bb reached_cont reached_state)" 
+  shows "(Ast.valid_configuration A \<Lambda>1_local \<Gamma> \<Omega> nested_loop2_before_ast_cfg.post reached_bb reached_cont reached_state)"
+  apply (rule ending_after_unwrapping)
+     apply (rule j_step_ast_trace)
+    apply (simp add: loop1_body_bb1_def)
+    apply (rule cfg_is_correct, simp)
+   apply (rule cfg_satisfies_post, blast)
+   apply simp
+  apply (rule loop1_body_bb1_unwrapped_global_rel)
+    apply (simp add: loop1_body_bb1_unwrapped_def)
+    apply assumption
+   apply blast
+  apply (rule loop_ih)
+    apply (rule strictly_smaller_helper2)
+     apply assumption+
+  done
+
+lemma bb0_unwrapped_global_rel:
   assumes j_step_ast_trace: 
     "A,M,\<Lambda>1_local,\<Gamma>,\<Omega>,T \<turnstile> (bb0_unwrapped, KEndBlock KStop, Normal ns1) -n\<longrightarrow>^j (reached_bb, reached_cont, reached_state)"
-  and cfg_is_correct: "\<And> m' s'. (red_cfg_multi A M \<Lambda>1_local \<Gamma> \<Omega> nested_loop2_before_cfg_to_dag_prog.proc_body ((Inl 3),(Normal ns1)) (m',s')) \<Longrightarrow> (s' \<noteq> Failure)"
-  shows "(Ast.valid_configuration A \<Lambda>1_local \<Gamma> \<Omega> [] reached_bb reached_cont reached_state)"
+  and cfg_is_correct: "\<And> m' s'. (red_cfg_multi A M \<Lambda>1_local \<Gamma> \<Omega> nested_loop2_before_cfg_to_dag_prog.proc_body ((Inl 1),(Normal ns1)) (m',s')) \<Longrightarrow> (s' \<noteq> Failure)"
+  and cfg_satisfies_post: "\<And>m' s'.
+                           (A,M,\<Lambda>1_local,\<Gamma>,\<Omega>,nested_loop2_before_cfg_to_dag_prog.proc_body \<turnstile>(Inl 1, Normal ns1) -n\<rightarrow>* (m', s')) \<Longrightarrow>
+                           is_final_config (m', s') \<Longrightarrow> (\<forall>ns_end. s' = Normal ns_end \<longrightarrow> list_all (expr_sat A \<Lambda>1_local \<Gamma> \<Omega> ns_end) nested_loop2_before_ast_cfg.post)"
+  shows "(Ast.valid_configuration A \<Lambda>1_local \<Gamma> \<Omega> nested_loop2_before_ast_cfg.post reached_bb reached_cont reached_state)"
   using assms 
 proof (induction j arbitrary: ns1 rule: less_induct)
   case (less j)
@@ -393,6 +626,7 @@ proof (induction j arbitrary: ns1 rule: less_induct)
               apply (simp add: bb0_unwrapped_def)
              apply (rule less(2))
             apply (rule less(3), simp)
+           apply (rule less(4), blast)
            apply simp
            apply (simp add: bb0_unwrapped_def)
           apply simp
@@ -401,33 +635,41 @@ proof (induction j arbitrary: ns1 rule: less_induct)
               apply (simp add: bb0_unwrapped_def)
             apply (simp add: bb0_unwrapped_def)
            apply (simp, simp, simp)
-       apply (simp add: nested_loop2_before_cfg_to_dag_prog.node_3)
-       apply (simp add: nested_loop2_before_cfg_to_dag_prog.block_3_def)
+       apply (simp add: nested_loop2_before_cfg_to_dag_prog.node_1)
+       apply (simp add: nested_loop2_before_cfg_to_dag_prog.block_1_def)
       apply(rule disjE)
         apply assumption
     
-       apply (erule allE[where x = 4])
-       apply (simp add: nested_loop2_before_cfg_to_dag_prog.outEdges_3)
+       apply (erule allE[where x = 2])+
+       apply (simp add: nested_loop2_before_cfg_to_dag_prog.outEdges_1)
        apply (simp add:member_rec(1))
        apply (rule conjE)
         apply assumption
        apply simp
-       apply (rule inner_loop_head_global_rel_wrapped)
-         apply (simp add: outer_body_bb1_def outer_body_bb2_def)
+       apply (rule loop1_body_bb1_wrapped_global_rel)
+         apply (simp add: loop1_body_bb1_def)
         apply (rule correctness_propagates_through_assumption2)
             apply assumption
-           apply (simp add: nested_loop2_before_cfg_to_dag_prog.node_4)
-           apply (simp add: nested_loop2_before_cfg_to_dag_prog.block_4_def)
+           apply (simp add: nested_loop2_before_cfg_to_dag_prog.node_2)
+           apply (simp add: nested_loop2_before_cfg_to_dag_prog.block_2_def)
           apply assumption
-         apply (simp add: nested_loop2_before_cfg_to_dag_prog.outEdges_4)
+         apply (simp add: nested_loop2_before_cfg_to_dag_prog.outEdges_2)
          apply (simp add: member_rec)
-        apply assumption
+         apply assumption
+        apply (rule correctness_propagates_through_assumption4)
+             apply blast
+            apply (simp add: nested_loop2_before_cfg_to_dag_prog.node_2)
+            apply (simp add: nested_loop2_before_cfg_to_dag_prog.block_2_def)
+           apply simp
+          apply (simp add: nested_loop2_before_cfg_to_dag_prog.outEdges_2)
+          apply (simp add: member_rec)
+         apply simp+
        apply (rule less.IH)
          apply (rule strictly_smaller_helper2)
           apply assumption+
 
-      apply (erule allE[where x = 8])
-      apply (simp add:nested_loop2_before_cfg_to_dag_prog.outEdges_3)
+      apply (erule allE[where x = 9])+
+      apply (simp add:nested_loop2_before_cfg_to_dag_prog.outEdges_1)
       apply (simp add:member_rec(1))
       apply (rule conjE)
        apply assumption
@@ -437,10 +679,13 @@ proof (induction j arbitrary: ns1 rule: less_induct)
           apply simp
          apply simp
          apply blast
+        apply blast
         apply simp
        apply simp
       apply (rule end_global_rel)
-        apply (simp add: empty_bb_def)+
+         apply (simp add: empty_bb_def)
+        apply simp
+       apply assumption+
       done
   qed
 qed
@@ -448,28 +693,36 @@ qed
 lemma entry_block_global_rel:
   assumes j_step_ast_trace: "A,M,\<Lambda>1_local,\<Gamma>,\<Omega>,T \<turnstile> (bigblock0, KStop, Normal ns1) -n\<longrightarrow>^j (reached_bb, reached_cont, reached_state)"
   and cfg_is_correct: "\<And> m' s'. (red_cfg_multi A M \<Lambda>1_local \<Gamma> \<Omega> nested_loop2_before_cfg_to_dag_prog.proc_body ((Inl 0),(Normal ns1)) (m',s')) \<Longrightarrow> (s' \<noteq> Failure)"
-  shows "(Ast.valid_configuration A \<Lambda>1_local \<Gamma> \<Omega> nested_loop2_before_cfg_to_dag_prog.post reached_bb reached_cont reached_state)"
+  and cfg_satisfies_post: "\<And>m' s'.
+                           (A,M,\<Lambda>1_local,\<Gamma>,\<Omega>,nested_loop2_before_cfg_to_dag_prog.proc_body \<turnstile>(Inl 0, Normal ns1) -n\<rightarrow>* (m', s')) \<Longrightarrow>
+                           is_final_config (m', s') \<Longrightarrow> (\<forall>ns_end. s' = Normal ns_end \<longrightarrow> list_all (expr_sat A \<Lambda>1_local \<Gamma> \<Omega> ns_end) nested_loop2_before_ast_cfg.post)"
+  shows "(Ast.valid_configuration A \<Lambda>1_local \<Gamma> \<Omega> nested_loop2_before_ast_cfg.post reached_bb reached_cont reached_state)"
   using assms
 proof -
   show ?thesis
-    unfolding nested_loop2_before_cfg_to_dag_prog.post_def
     apply (rule block_global_rel_while_successor)
            apply (rule j_step_ast_trace)
           apply (rule Rel_Main_test[of bigblock0 _ nested_loop2_before_cfg_to_dag_prog.block_0])
+            apply (simp add: bigblock0_def nested_loop2_before_cfg_to_dag_prog.block_0_def)
+           apply (simp add: bigblock0_def nested_loop2_before_cfg_to_dag_prog.block_0_def)
           apply (simp add: bigblock0_def nested_loop2_before_cfg_to_dag_prog.block_0_def)
-         apply (simp add: bigblock0_def nested_loop2_before_cfg_to_dag_prog.block_0_def)
         apply (simp add: nested_loop2_before_cfg_to_dag_prog.block_0_def)
        apply (rule disjI1)
        apply (rule nested_loop2_before_cfg_to_dag_prog.node_0)
        apply (rule cfg_is_correct, simp)
+      apply (rule cfg_satisfies_post, blast)
       apply simp
      apply (simp add: nested_loop2_before_cfg_to_dag_prog.node_0)
      apply (rule bb0_local_rel)
       apply assumption
      apply simp
-    apply (rule outer_loop_head_global_rel)
-     apply (simp add: bb0_unwrapped_def)
+    apply (erule allE[where x = 1])+
     apply (simp add: nested_loop2_before_cfg_to_dag_prog.outEdges_0)
     apply (simp add: member_rec(1))
+    apply (rule bb0_unwrapped_global_rel)
+     apply (simp add: bb0_unwrapped_def)
+    apply blast+
     done
 qed
+
+end
